FunProg
- Notations
- Simplification

FunProg.v
@@ -30,10 +30,36 @@ Module Spec.
     Qed.
   End WLP.
 
-  Record t (A : DTuple.p) := {
-    pre  : Prop;
-    post : DTuple.arrow A (fun _ => pre -> Prop);
+  Record t (A : DTuple.p) := mk_t {
+    pre_p  : option Prop;
+    post_p : option (OptProp.arrow pre_p (fun _ => DTuple.arrow A (fun _ => Prop)));
   }.
+  Global Arguments mk_t [A] _ _.
+
+  Definition pre [A] (s : t A) : Prop :=
+    OptProp.t (pre_p s).
+
+  Definition post_o [A] (s : t A) (PRE : pre s) (res : DTuple.t A) : option Prop :=
+    option_map (fun post => DTuple.to_fun (OptProp.to_fun post PRE) res) (post_p s).
+
+  Definition post [A] (s : t A) (PRE : pre s) (res : DTuple.t A) : Prop :=
+    OptProp.t (post_o s PRE res).
+
+  Definition pull_f [A B] (f : DTuple.t A -> DTuple.t B) (s : Spec.t B) : Spec.t A :=
+    Spec.mk_t (Spec.pre_p s)
+      (option_map (fun post => OptProp.of_fun (fun PRE => DTuple.of_fun (fun x =>
+                               DTuple.to_fun (OptProp.to_fun post PRE) (f x))))
+                  (Spec.post_p s)).
+  Global Arguments pull_f _ _ _ !_/.
+
+  Lemma pull_f_post [A B] f s PRE x:
+    post (@pull_f A B f s) PRE x <-> post s PRE (f x).
+  Proof.
+    unfold pull_f, post, post_o; cbn.
+    case post_p as [|]; cbn;
+    try rewrite OptProp.to_of_fun, DTuple.to_of_fun;
+    reflexivity.
+  Qed.
 End Spec.
 
 
@@ -102,9 +128,45 @@ Section Instr.
     reflexivity.
   Qed.
 
-  Program Definition Call [A : DTuple.p] (s : Spec.t A) : instr (DTuple.Pcons (Spec.pre s) (fun _ => A))
+  Section CallRet.
+    Variables (pre : OptProp.p) (A : DTuple.p).
+
+    Definition Call_ret :=
+      match pre with
+      | Some pre => DTuple.Pcons pre (fun _ => A)
+      | None     => A
+      end.
+
+    Definition to_Call_ret : OptProp.t pre * DTuple.t A -> DTuple.t Call_ret.
+    Proof.
+      unfold Call_ret; case pre as [|]; cbn.
+      - exact (fun '(PRE, x) => DTuple.pair PRE x).
+      - exact (fun '(_, x) => x).
+    Defined.
+
+    Definition of_Call_ret : DTuple.t Call_ret -> OptProp.t pre * DTuple.t A.
+    Proof.
+      unfold Call_ret; case pre as [|]; cbn.
+      - intros [PRE x]. exact (PRE, x).
+      - exact (fun x => (I, x)).
+    Defined.
+
+    Lemma iso_Call_ret :
+      type_iso (OptProp.t pre * DTuple.t A) (DTuple.t Call_ret)
+        to_Call_ret of_Call_ret.
+    Proof.
+      unfold Call_ret, to_Call_ret, of_Call_ret.
+      split; case pre as [|]; cbn;
+      repeat (let x := fresh "x" in intro x; try (case x; clear x)); reflexivity.
+    Qed.
+  End CallRet.
+  Global Arguments to_Call_ret [_ _].
+  Global Arguments of_Call_ret [_ _].
+
+  Program Definition Call [A : DTuple.p] (s : Spec.t A)
+    : instr (Call_ret (Spec.pre_p s) A)
     := fun post => exists PRE : Spec.pre s, forall x : DTuple.t A,
-      DTuple.to_fun (Spec.post s) x PRE -> post (DTuple.pair PRE x).
+       Spec.post s PRE x -> post (to_Call_ret (PRE, x)).
   Next Obligation.
     intros [PRE].
     exists PRE; auto.
@@ -134,8 +196,8 @@ Section WLP_Formula.
     apply F; auto.
   Qed.
 
-  Lemma wlp_formula_def [A] i:
-    @wlp_formula A i (wlp i).
+  Lemma wlp_formula_Ret [A] x:
+    wlp_formula (@Ret A x) (fun post => post x).
   Proof.
     constructor; auto.
   Qed.
@@ -155,11 +217,23 @@ Section WLP_Formula.
 
   Lemma wlp_formula_Call [A] s:
     wlp_formula (@Call A s)
-      (fun post => exists PRE : Spec.pre s,
-        DTuple.all A (fun x => DTuple.to_fun (Spec.post s) x PRE ->
-        post (DTuple.pair PRE x))).
+      (fun post =>
+        OptProp.ex (Spec.pre_p s) (fun PRE =>
+        DTuple.all A (fun x =>
+        OptProp.all (Spec.post_o s PRE x) (fun _ =>
+        post (to_Call_ret (PRE, x)))))).
   Proof.
-    constructor; setoid_rewrite DTuple.all_iff; auto.
+    constructor.
+    setoid_rewrite OptProp.ex_iff.
+    setoid_rewrite DTuple.all_iff.
+    setoid_rewrite OptProp.all_iff.
+    auto.
+  Qed.
+
+  Lemma wlp_formula_Assert P:
+    wlp_formula (Assert P) (fun post => P /\ post DTuple.tt).
+  Proof.
+    constructor; auto.
   Qed.
 End WLP_Formula.
 
@@ -186,7 +260,7 @@ Ltac case_2heads x f a b :=
 (* build a formula [match x with ... end] *)
 Ltac build_wlp_formula_match build_f x :=
   lazymatch goal with |- wlp_formula _ ?f =>
-  Tac.build_term f ltac:(fun _ => intro (* post *); case x; shelve)
+  Tac.build_term f ltac:(fun _ => intro (* post *); case x as []; shelve)
   end;
   cbn;
   lazymatch goal with |- @wlp_formula ?A ?i ?f =>
@@ -229,14 +303,14 @@ Ltac build_wlp_formula_ dmatch :=
   cbn; clear;
   lazymatch goal with
   | |- wlp_formula (Ret _) _ =>
-      refine (wlp_formula_def _)
+      refine (wlp_formula_Ret _)
   | |- wlp_formula (Bind _ _) _ =>
       refine (wlp_formula_Bind _ _);
       [ build | cbn; repeat intro; build ]
   | |- wlp_formula (@Call ?A ?s) _ =>
       exact (@wlp_formula_Call A s)
   | |- wlp_formula (Assert _) _ =>
-      refine (wlp_formula_def _)
+      refine (wlp_formula_Assert _)
   | |- wlp_formula (match ?x with _ => _ end) _ =>
       lazymatch dmatch with
       | true =>
@@ -308,36 +382,54 @@ Ltac solve_wlp :=
       end
   end.
 
+Ltac solve_by_wlp :=
+  by_wlp_ false;
+  solve_wlp;
+  eauto.
+
 (* Program simplification *)
 
 Section SimplCont.
-  Inductive k_opt (A : DTuple.p) : forall B : DTuple.p, Type :=
-    | KNone : k_opt A A
-    | KSome [B : DTuple.p] (k : DTuple.arrow A (fun _ => instr B)) : k_opt A B.
-  Global Arguments KNone {_}.
-  Global Arguments KSome [_ _].
+  Inductive k_t (A B : DTuple.p) :=
+    mk_k (C : DTuple.p)
+         (f : DTuple.t A -> DTuple.t C)
+         (k : DTuple.arrow C (fun _ => instr B)).
+  Global Arguments mk_k [_ _].
 
-  Definition k_apply [A B] (i : instr A) (k : k_opt A B) : instr B :=
-    match k with
-    | KNone   => i
-    | KSome k => Bind i k
-    end.
+  Definition k_pull_f [A B C] (f : DTuple.t A -> DTuple.t B) : k_t B C -> k_t A C :=
+    fun '(mk_k _ f' k) =>
+    mk_k _ (fun x => f' (f x)) k.
+
+  Definition k_fk [A B] (k : k_t A B) (x : DTuple.t A) : instr B :=
+    let '(mk_k _ f k) := k in
+    DTuple.to_fun k (f x).
+  Global Arguments k_fk [_ _] !k/.
+
+  Definition k_apply [A B] (i : instr A) (k : k_t A B) : instr B :=
+    Bind i (DTuple.of_fun (k_fk k)).
+  Global Arguments k_apply [_ _] i !k/.
 
   Local Add Parametric Morphism A B : (@k_apply A B)
-    with signature (@eqv A) ==> (@eq (k_opt A B)) ==> (@eqv B)
+    with signature (@eqv A) ==> (@eq (k_t A B)) ==> (@eqv B)
     as k_apply_morh.
   Proof.
-    intros i0 i1 E [|k]; cbn; rewrite E; reflexivity.
+    intros i0 i1 E k; unfold k_apply; rewrite E; reflexivity.
   Qed.
 
-  Inductive simpl_cont [A B] (i : instr A) (k : k_opt A B) (r : instr B) : Prop :=
+  Inductive simpl_cont [A B] (i : instr A) (k : k_t A B) (r : instr B) : Prop :=
     simpl_contI (E : eqv r (k_apply i k)).
 
+  Definition k_None {A : DTuple.p} : k_t A A :=
+    mk_k A (fun x => x) (DTuple.of_fun (@Ret A)).
+
   Lemma eqv_by_simpl_cont [A i0 i1]
-    (S : @simpl_cont A A i0 KNone i1):
+    (S : @simpl_cont A A i0 k_None i1):
     eqv i0 i1.
   Proof.
-    symmetry; apply S.
+    case S as [->].
+    intro; cbn.
+    apply (Spec.wp_morph (wlp_monotone _)).
+    intro; rewrite !DTuple.to_of_fun; reflexivity.
   Qed.
 
   Lemma simpl_cont_morph [A B i0 i1] k
@@ -356,74 +448,186 @@ Section SimplCont.
   Qed.
 
   Lemma simpl_cont_Ret [A B] x k:
-    @simpl_cont A B (Ret x) (KSome k) (DTuple.to_fun k x).
+    @simpl_cont A B (Ret x) k (k_fk k x).
   Proof.
-    constructor; intro; reflexivity.
+    case k as []; constructor; intro; cbn.
+    rewrite DTuple.to_of_fun; reflexivity.
   Qed.
 
-  Lemma simpl_cont_Bind [A B C f0 f1 g0 g1 k]
+
+  Lemma simpl_cont_Call_pre [A B post k r]
+    (C : simpl_cont (Call (Spec.mk_t None (option_map (fun post => post Logic.I) post)))
+          (k_pull_f (A := A) (B := DTuple.Pcons _ _) (fun x => DTuple.pair Logic.I x) k) r):
+    @simpl_cont _ B (@Call A (Spec.mk_t (Some True) post)) k r.
+  Proof.
+    constructor. etransitivity. apply C.
+    intro; unfold k_pull_f, k_apply, k_fk; case k as []; cbn.
+    apply Morphisms_Prop.ex_iff_morphism; intros [].
+    case post; cbn; reflexivity.
+  Qed.
+
+  Lemma simpl_cont_Call_post [A B pre k r]
+    (C : simpl_cont (Call (Spec.mk_t pre None)) k r):
+    @simpl_cont _ B
+      (@Call A (Spec.mk_t pre (Some (OptProp.of_fun (fun _ => DTuple.of_fun (fun _ => True)))))) k r.
+  Proof.
+    constructor. etransitivity. apply C.
+    intro; unfold k_apply, k_fk; case k as []; cbn.
+    apply Morphisms_Prop.ex_iff_morphism;  intro.
+    apply Morphisms_Prop.all_iff_morphism; intro.
+    rewrite OptProp.to_of_fun, !DTuple.to_of_fun.
+    reflexivity.
+  Qed.
+
+  Definition k_pull_f_Call [A A' B] (s : Spec.t A) (f : DTuple.t A' -> DTuple.t A)
+    (k : k_t (Call_ret (Spec.pre_p s) A) B) :
+    k_t (Call_ret (Spec.pre_p s) A') B.
+  Proof.
+    refine (k_pull_f _ k).
+    cbn.
+    intros [PRE x]%of_Call_ret.
+    exact (to_Call_ret (PRE, f x)).
+  Defined.
+  Global Arguments k_pull_f_Call _ _ _ _ _ _/.
+
+  Lemma simpl_cont_Call [A A' B s k rf rg r]
+    (Ru : DTuple.iso_p A A' rf rg)
+    (C : simpl_cont (@Call A' (Spec.pull_f rg s)) (k_pull_f_Call s rg k) r):
+    @simpl_cont _ B (@Call A s) k r.
+  Proof.
+    constructor. etransitivity. apply C.
+    destruct k, Ru as [[R0 R1]]; cbn.
+    intro; unfold k_pull_f_Call, k_apply, k_fk; cbn.
+    apply Morphisms_Prop.ex_iff_morphism; intro PRE.
+    setoid_rewrite Spec.pull_f_post.
+    split; intros H x;
+    [ generalize (H (rf x)) | generalize (H (rg x)) ];
+    clear H; rewrite !DTuple.to_of_fun, (proj1 (iso_Call_ret _ _)), ?R0, ?R1;
+    exact (fun H => H).
+  Qed.
+
+  Lemma simpl_cont_Bind [A A' B C f0 f1 g0 g1 k rf rg]
     (Eg : DTuple.arrow A (fun x =>
             @simpl_cont B C (DTuple.to_fun g0 x) k (DTuple.to_fun g1 x)))
-    (Ef : @simpl_cont A C f0 (KSome g1) f1):
+    (Ru : DTuple.iso_p A A' rf rg)
+    (Ef : @simpl_cont A C f0 (mk_k A' rf (DTuple.of_fun (fun x => DTuple.to_fun g1 (rg x)))) f1):
     @simpl_cont B C (Bind f0 g0) k f1.
   Proof.
     constructor.
     etransitivity. apply Ef.
-    cbn.
+    cbn [k_apply k_fk].
     etransitivity. apply Bind_morph. reflexivity.
-    { intro x. etransitivity. apply (DTuple.to_fun Eg x).
-      apply R_refl. reflexivity.
-      symmetry. exact (DTuple.to_of_fun _ x). }
-    clear.
-    case k as [|k]; cbn.
-    - apply Bind_morph. reflexivity.
-      intro; rewrite DTuple.to_of_fun. reflexivity.
-    - symmetry; apply Bind_assoc.
+    - intro x. etransitivity.
+      + rewrite !DTuple.to_of_fun.
+        case Ru as [[->]].
+        apply (DTuple.to_fun Eg).
+      + apply R_refl. reflexivity.
+        symmetry. exact (DTuple.to_of_fun _ x).
+    - clear.
+      case k as [].
+      symmetry; apply Bind_assoc.
+  Qed.
+
+  Lemma simpl_cont_branch [A B C i r f k]
+    (S : simpl_cont i (mk_k C f (DTuple.of_fun (fun x => Ret x))) r):
+    @simpl_cont A B i (mk_k C f k) (Bind r k).
+  Proof.
+    constructor.
+    case S; cbn [k_apply k_fk]; intros ->.
+    rewrite Bind_assoc.
+    apply Bind_morph; [reflexivity|intro].
+    rewrite !DTuple.to_of_fun.
+    intro; reflexivity.
   Qed.
 End SimplCont.
 
 Ltac build_simpl_cont :=
-  let rec build _ :=
-    cbn;
-    lazymatch goal with
-    | |- simpl_cont (Ret _) (KSome _) _ =>
-        refine (simpl_cont_Ret _ _)
-    | |- simpl_cont (Ret _) KNone _ =>
-        refine (simpl_cont_def _ _)
-    | |- simpl_cont (Bind _ _) _ _ =>
-        refine (simpl_cont_Bind _ _);
-        [ cbn; repeat intro; build tt
-        | build tt]
-    | |- simpl_cont (Call _) _ _ =>
-        refine (simpl_cont_def _ _)
-    | |- simpl_cont (Assert _) _ _ =>
-        refine (simpl_cont_def _ _)
-    | |- simpl_cont (match ?x with _ => _ end) _ ?r =>
-        tryif Tac.is_single_case x
-        then (
-          Tac.build_term r ltac:(fun tt => case x; shelve);
-          cbn;
-          lazymatch goal with |- @simpl_cont ?A ?B ?i ?k ?r =>
-          let i' := fresh "i" in
-          case_2heads x (fun i' => @simpl_cont A B i' k) i r
-          end;
-          build tt
-        ) else (
-          refine (simpl_cont_morph _ _);
-          lazymatch goal with |- eqv _ ?r =>
-          Tac.build_term r ltac:(fun _ => case x; shelve)
-          end;
-          lazymatch goal with |- @eqv ?A ?i ?r =>
-          case_2heads x (@eqv A) i r
-          end;
-          refine (eqv_by_simpl_cont _); build tt
-        )
-    | |- ?g => fail "build_simpl_cont" g
-    end
-  in build tt.
+  cbn;
+  lazymatch goal with
+  | |- simpl_cont (Ret _) _ _ =>
+      refine (simpl_cont_Ret _ _)
+  | |- simpl_cont (Bind _ _) _ _ =>
+      refine (simpl_cont_Bind _ _ _);
+      [ cbn; repeat intro; build_simpl_cont
+      | DTuple.build_iso_p_remove_unit
+      | build_simpl_cont ]
+  | |- @simpl_cont _ ?B (@Call ?A ?s) ?k _ =>
+      refine (@simpl_cont_Call A _ B s k _ _ _ _ _);
+      [ DTuple.build_iso_p_remove_unit |
+      cbn;
+      try lazymatch goal with |- @simpl_cont _ ?B (@Call ?A ?s) ?k _ =>
+      refine (@simpl_cont_Call_pre A B _ k _ _);
+      cbn
+      end;
+      try lazymatch goal with |- @simpl_cont _ ?B (@Call ?A (Spec.mk_t ?pre _)) ?k _ =>
+      refine (@simpl_cont_Call_post A B pre k _ _);
+      cbn
+      end;
+      refine (simpl_cont_def _ _) ]
+  | |- simpl_cont (Assert _) _ _ =>
+      refine (simpl_cont_def _ _)
+  | |- simpl_cont (match ?x with _ => _ end) _ _ =>
+      (tryif Tac.is_single_case x
+       then idtac
+       else refine (simpl_cont_branch _));
+      lazymatch goal with |- simpl_cont _ _ ?r =>
+      Tac.build_term r ltac:(fun tt => case x as []; shelve);
+      cbn
+      end;
+      lazymatch goal with |- @simpl_cont ?A ?B ?i ?k ?r =>
+      let i' := fresh "i" in
+      case_2heads x (fun i' => @simpl_cont A B i' k) i r
+      end;
+      build_simpl_cont
+  | |- ?g => fail "build_simpl_cont" g
+  end.
 
 Ltac simpl_prog :=
   refine (wlpA_eqv _ _);
   [ refine (eqv_by_simpl_cont _);
     build_simpl_cont
   | cbn ].
+
+Global Opaque Ret Bind Call Assert.
+
+Module Notations.
+  Export DTuple.Notations.
+
+  Notation "f ;; g" :=
+    (@Bind DTuple.Pnil _ f g)
+    (at level 199, right associativity, only printing,
+     format "f ;; '//' g").
+
+  Notation "'let' x .. y <- f ; g" :=
+    (Bind f (fun x => .. (fun y => g) ..))
+    (at level 200, x closed binder, y closed binder, right associativity, only printing,
+     format "'[' 'let'  '[' x  ..  y  <-  ']' '/  ' f ; '//' g ']'").
+
+  Notation "'return' x" :=
+    (Ret x)
+    (at level 100, x at level 0, only printing).
+
+  Notation "'call' ( 'req' : pre ) ( 'ens' x .. y : post )" :=
+    (Call {| Spec.pre_p := Some pre; Spec.post_p := Some (fun x => .. (fun y => post) .. ) |})
+    (at level 100, pre at level 200, x closed binder, y closed binder, post at level 200, only printing,
+     format "'call'  '[hv' ( 'req'  :  pre )  '/' ( '[  ' 'ens'  '[' x  ..  y  :  ']' post ']' ) ']'").
+
+  Notation "'call' ( 'ens' x .. y : post )" :=
+    (Call {| Spec.pre_p := None; Spec.post_p := Some (fun x => .. (fun y => post) .. ) |})
+    (at level 100, x closed binder, y closed binder, post at level 200, only printing,
+     format "'call'  ( '[  ' 'ens'  '[' x  ..  y  :  ']' post ']' )").
+
+  Notation "'call' ( 'ens' : post )" :=
+    (Call {| Spec.pre_p := None; Spec.post_p := Some post |})
+    (at level 100, post at level 200, only printing,
+     format "'call'  ( '[  ' 'ens'  :  post ']' )").
+
+  Notation "'call' ( 'req' : pre )" :=
+    (Call {| Spec.pre_p := Some pre; Spec.post_p := None |})
+    (at level 100, pre at level 200, only printing,
+     format "'call'  ( 'req'  :  pre )").
+
+  Notation "'call'" :=
+    (Call {| Spec.pre_p := None; Spec.post_p := None |})
+    (at level 100, only printing).
+End Notations.
